Updated kruskal files: Added missing sample_mark/unionfind_arr.h Added extra lemmas in undirected_graph Verified init_empty_graph Removed binary_heap from kruskal, re-added sorting instead

kruskal/WeightedEdgeListGraph.v
@@ -1,6 +1,5 @@
 (*Looted from msl_application/DijkstraArrayGraph
 Should try abstracting it if possible from an EdgeListGraph*)
-Require Export VST.floyd.proofauto.
 Require Import Coq.ZArith.ZArith.
 Require Import Coq.micromega.Lia.
 Require Import VST.msl.seplog.
@@ -10,6 +9,7 @@ Require Import RamifyCoq.lib.Coqlib.
 Require Import RamifyCoq.lib.EquivDec_ext.
 Require Import RamifyCoq.lib.List_ext.
 Require Import RamifyCoq.graph.graph_model.
+Require Import RamifyCoq.graph.graph_gen.
 (*Require Import RamifyCoq.msl_application.ArrayGraph.*) (*I probably need this to transform this graph to the ArrayGraph?*)
 Require Import RamifyCoq.graph.FiniteGraph.
 Require Import Coq.Lists.List.
@@ -23,9 +23,6 @@ Local Open Scope Z_scope.
 Instance Z_EqDec : EqDec Z eq. Proof. hnf. intros. apply Z.eq_dec. Defined.
 
 Definition is_null_Z: DecidablePred Z := existT (fun P : Z -> Prop => forall a : Z, {P a} + {~ P a}) (fun x : Z => x < 0) (fun a : Z => Z_lt_dec a 0).
-
-(*Definition SIZE := 8.
-Definition IFTY := Int.max_signed - Int.max_signed / SIZE.*)
 
 (*
  Concretizing the EdgelistGraph with array-specific types.
@@ -53,30 +50,101 @@ Proof.
   - right; intro; apply c; inversion H; reflexivity.
 Defined.
 
-Definition LGraph := LabeledGraph VType EType LV LE LG.
+Definition WEdgeListGraph := LabeledGraph VType EType LV LE LG.
+(*
+Print Build_PreGraph.
+Print Build_LabeledGraph.
 
-Class Fin (g: LGraph) :=
+Definition Build_WEdgeListGraph := Build_LabeledGraph LV LE LG.
+*)
+
+Class Fin (g: WEdgeListGraph) :=
   { fin: FiniteGraph g; }.
 
-Definition Graph := (GeneralGraph VType EType LV LE LG (fun g => Fin g)).
+Definition FiniteWEdgeListGraph := (GeneralGraph VType EType LV LE LG (fun g => Fin g)).
 
-Definition src_edge (g: LGraph): Prop :=
+Definition src_edge (g: WEdgeListGraph): Prop :=
   forall e, src g e = fst e.
 
-Definition dst_edge (g: LGraph): Prop :=
+Definition dst_edge (g: WEdgeListGraph): Prop :=
   forall e, dst g e = snd e.
 
-Definition vertex_valid (g: LGraph): Prop :=
-  forall v, vvalid g v <-> 0 <= v < Int.max_signed.
+Definition vertex_valid (g: WEdgeListGraph): Prop :=
+  forall v, vvalid g v -> 0 <= v < Int.max_signed.
 
-Definition edge_valid (g: LGraph): Prop :=
-  forall a b, evalid g (a,b) <-> (vvalid g a /\ vvalid g b).
+Definition edge_valid (g: WEdgeListGraph): Prop :=
+  forall a b, evalid g (a,b) -> (vvalid g a /\ vvalid g b).
 
-Definition weight_valid (g: LGraph): Prop :=
+Definition weight_valid (g: WEdgeListGraph): Prop :=
   forall e, evalid g e -> Int.min_signed <= elabel g e <= Int.max_signed. (*< IFTY*)
 
-Definition sound_weighted_edge_graph (g: LGraph): Prop :=
+Definition sound_weighted_edge_graph (g: WEdgeListGraph): Prop :=
   vertex_valid g /\ edge_valid g /\ src_edge g /\ dst_edge g /\ weight_valid g.
+
+Definition numV (g: WEdgeListGraph) {fg : FiniteGraph g} : Z := Zlength (VList g).
+Definition numE (g: WEdgeListGraph) {fg : FiniteGraph g} : Z := Zlength (EList g).
+
+(* from Graph to list of edges *)
+Definition graph_to_wedgelist (g: WEdgeListGraph) {fg: FiniteGraph g} : list (LE*EType) :=
+  map (fun e => (elabel g e, e)) (EList g). (*ordering?*)
+
+
+(*Example of a WEdgeListGraph (returned by init_empty_graph*)
+(*ASDF: Change this into a FiniteWEdgeListGraph (the generalgraph as defined above)
+so we don't have to lug {FiniteGraph g} around *)
+Definition empty_WEdgeListGraph : WEdgeListGraph :=
+(empty_labeledgraph (fun e => fst e) (fun e => snd e) tt 0 tt).
+
+Definition empty_WEdgeListGraph_finite:
+  FiniteGraph empty_WEdgeListGraph.
+Proof.
+constructor; unfold EnumEnsembles.Enumerable, In; exists nil; split; intros; simpl.
+apply NoDup_nil. reflexivity. apply NoDup_nil. reflexivity.
+Qed.
+
+Lemma empty_WEdgeListGraph_sound:
+  sound_weighted_edge_graph empty_WEdgeListGraph.
+Proof.
+repeat split; try contradiction.
+Qed.
+
+Lemma empty_WEdgeListGraph_VList {fg: FiniteGraph empty_WEdgeListGraph}:
+  VList empty_WEdgeListGraph = nil.
+Proof.
+unfold VList. destruct fg. simpl in finiteV. unfold EnumEnsembles.Enumerable in finiteV.
+destruct finiteV. destruct a.
+unfold proj1_sig. unfold finiteV.
+destruct x. reflexivity.
+assert (In v (v::x)) by (apply in_eq). specialize i with v. destruct i. contradiction.
+Qed.
+
+Lemma empty_WEdgeListGraph_EList {fg: FiniteGraph empty_WEdgeListGraph}:
+  EList empty_WEdgeListGraph = nil.
+Proof.
+unfold EList. destruct fg. simpl in finiteE; unfold EnumEnsembles.Enumerable in finiteE.
+destruct finiteE. destruct a.
+unfold proj1_sig; unfold finiteE.
+destruct x. reflexivity.
+assert (In e (e::x)) by (apply in_eq). specialize i with e. destruct i. contradiction.
+Qed.
+
+Corollary empty_WEdgeListGraph_numV {fg: FiniteGraph empty_WEdgeListGraph}:
+  numV empty_WEdgeListGraph = 0.
+Proof.
+unfold numV. rewrite empty_WEdgeListGraph_VList. apply Zlength_nil.
+Qed.
+
+Corollary empty_WEdgeListGraph_numE {fg: FiniteGraph empty_WEdgeListGraph}:
+  numE empty_WEdgeListGraph = 0.
+Proof.
+unfold numE. rewrite empty_WEdgeListGraph_EList. apply Zlength_nil.
+Qed.
+
+Corollary empty_WEdgeListGraph_graph_to_wedgelist {fg: FiniteGraph empty_WEdgeListGraph}:
+  graph_to_wedgelist empty_WEdgeListGraph = nil.
+Proof.
+unfold graph_to_wedgelist. rewrite empty_WEdgeListGraph_EList. reflexivity.
+Qed.
 
 (* Moving on to Spatial Rep *)
 
@@ -98,14 +166,8 @@ Section SpatialWEdgeListGraph.
   Context {SAGP: SpatialWEdgeListGraphAssum Pred}.
   Context {SAG: SpatialWEdgeListGraph Addr Pred}.
   
-  Definition numV (g: LGraph) {fg : FiniteGraph g} : Z := Zlength (VList g).
-  Definition numE (g: LGraph) {fg : FiniteGraph g} : Z := Zlength (EList g).
-
-  (* from Graph to list of edges *)
-  Definition graph_to_wedgelist (g: LGraph) {fg: FiniteGraph g} : list (LE*EType) :=
-    map (fun e => (elabel g e, e)) (EList g). (*ordering?*)
-
 End SpatialWEdgeListGraph.
+
 
 Lemma if_true_bool:
   forall (T : Type) (a : T) (b : bool) (c : T),
@@ -116,22 +178,3 @@ Lemma if_false_bool:
   forall (T : Type) (a : T) (b : bool) (c : T),
     b = false -> (if b then a else c) = c.
 Proof. intros. rewrite H. trivial. Qed.
-
-Lemma vvalid2_evalid:
-  forall g a b,
-    sound_weighted_edge_graph g ->
-    vvalid g a ->
-    vvalid g b ->
-    evalid g (a,b).
-Proof.
-  intros. destruct H as [_ [? _]].
-  red in H; rewrite H; split; trivial.
-Qed.
-
-Lemma vvalid_range:
-  forall g v,
-    sound_weighted_edge_graph g ->
-    vvalid g v <-> 0 <= v < Int.max_signed.
-Proof.
-  intros. destruct H as [? _]. red in H. trivial.
-Qed.
