kruskal/verif_kruskal_edgelist.v
@@ -1,33 +1,34 @@
+Require Import VST.floyd.proofauto.
 Require Import Coq.Lists.List.
 Require Import Coq.ZArith.ZArith.
 Require Import RamifyCoq.floyd_ext.share.
 Require Import RamifyCoq.lib.List_ext.
 Require Import RamifyCoq.graph.graph_model.
 (*are these needed?*)
-Require Import RamifyCoq.graph.path_lemmas.
+Require Import RamifyCoq.graph.path_lemmas. (*yes, because ufgraph relies on it*)
 Require Import RamifyCoq.graph.subgraph2.
 Require Import RamifyCoq.graph.graph_relation.
 Require Import RamifyCoq.graph.reachable_computable.
-(*edgelist*)
-Require Import RamifyCoq.kruskal.WeightedEdgeListGraph.
-Require Import RamifyCoq.kruskal.env_kruskal_edgelist.
-Require Import RamifyCoq.kruskal.spatial_wedgearray_graph.
 (*for unionfind*)
 Require Import RamifyCoq.graph.UnionFind.
 Require Import RamifyCoq.msl_application.UnionFindGraph.
 Require Import RamifyCoq.msl_application.ArrayGraph.
 Require Import RamifyCoq.sample_mark.env_unionfind_arr.
+(*edgelist*)
+Require Import RamifyCoq.kruskal.WeightedEdgeListGraph.
+Require Import RamifyCoq.kruskal.env_kruskal_edgelist.
+Require Import RamifyCoq.kruskal.spatial_wedgearray_graph.
 Require Import RamifyCoq.sample_mark.spatial_array_graph.
 (*spanning tree definition*)
 Require Import RamifyCoq.kruskal.mst.
 (*Require Import RamifyCoq.graph.spanning_tree.*)
-(*priority queue*)
-Require Import RamifyCoq.sample_mark.priorityqueue.
+
+Local Open Scope Z_scope.
 
 (*Taken from VST's queue*)
-Definition kruskal_mallocN_spec :=
- DECLARE kruskal_edgelist._mallocN
-  WITH sh:wshare, n: Z
+Definition mallocK_spec :=
+ DECLARE _mallocK
+  WITH sh: wshare, n: Z
   PRE [tint]
      PROP (4 <= n <= Int.max_unsigned)
      PARAMS (Vint (Int.repr n))
@@ -41,57 +42,141 @@ Definition kruskal_mallocN_spec :=
 
 (*It'll be useful if we can come up with some freeN spec, then centralize these in some header*)
 
-(* AM: You have a bug in the calls to graph_rep. *)
-
-(*
+(*overhaul this to explicitly return empty_WEdgeListGraph instead*)
 Definition init_empty_graph_spec :=
   DECLARE _kruskal
-  WITH sh: wshare
+  WITH gv: globals, sh: wshare
   PRE []
      PROP ()
      PARAMS ()
-     GLOBALS ()
-     SEP ()
+     GLOBALS (gv)
+     SEP (data_at sh tint (Vint (Int.repr MAX_EDGES)) (gv _MAX_EDGES))
   POST [ tptr t_wedgearray_graph ]
-     EX (g: WeightedEdgeListGraph.LGraph) {fg: FiniteGraph g},
-     EX pointer_g pointer_e: pointer_val,
-     PROP (sound_weighted_edge_graph g;
-           numV g = 0;
-           numE g = 0
-          )
-     LOCAL (temp ret_temp (pointer_val_val pointer_g))
-     SEP (graph_rep sh g (pointer_val_val pointer_g) (pointer_val_val pointer_e)).
+     EX {fg: FiniteGraph empty_WEdgeListGraph},
+     EX gptr eptr: pointer_val,
+     PROP ()
+     LOCAL (temp ret_temp (pointer_val_val gptr))
+     SEP (data_at sh tint (Vint (Int.repr MAX_EDGES)) (gv _MAX_EDGES) *
+          wedgearray_graph_rep sh empty_WEdgeListGraph gptr eptr).
 
-Instance CompSpecs : compspecs. Proof. make_compspecs prog. Defined.
 Definition Vprog : varspecs. mk_varspecs prog. Defined.
 Definition Gprog : funspecs := ltac:(with_library prog
-                                                  [kruskal_mallocN_spec; init_empty_graph_spec]).
+  [mallocK_spec; init_empty_graph_spec]).
 
 Lemma body_init_empty_graph: semax_body Vprog Gprog f_init_empty_graph init_empty_graph_spec.
 Proof.
 start_function.
-forward_call (sh, 12).
-(*yay what is this ._.*)
-set (j := Int64.max_unsigned) in *; compute in j; subst j.
-Abort.
+forward_call (sh, sizeof t_wedgearray_graph).
+set (j := Int.max_unsigned) in *; compute in j; subst j. simpl; lia.
+Intros gptr.
+assert (memory_block sh (sizeof t_wedgearray_graph) (pointer_val_val gptr) =
+        data_at_ sh (t_wedgearray_graph) (pointer_val_val gptr)). {
+  rewrite <- memory_block_data_at_; auto.
+} rewrite H0. clear H0.
+assert (data_at_ sh t_wedgearray_graph (pointer_val_val gptr) =
+        data_at sh t_wedgearray_graph (Vundef,(Vundef,Vundef)) (pointer_val_val gptr)). {
+  unfold data_at_, field_at_, data_at.
+  assert (default_val (nested_field_type t_wedgearray_graph []) = (Vundef,(Vundef,Vundef))) by reflexivity.
+  rewrite H0. auto.
+} rewrite H0. clear H0. (*that was easier than I thought :]*)
+forward.
+forward_call (sh, MAX_EDGES*(sizeof t_struct_edge)).
+set (j := Int.max_unsigned) in *; compute in j; subst j. simpl; lia.
+Intros eptr.
+assert (memory_block sh (MAX_EDGES * (sizeof t_struct_edge)) (pointer_val_val eptr) = data_at_ sh (tarray t_struct_edge MAX_EDGES) (pointer_val_val eptr)). {
+  assert (memory_block sh (MAX_EDGES*(sizeof t_struct_edge)) (pointer_val_val eptr) = memory_block sh (sizeof (tarray t_struct_edge MAX_EDGES)) (pointer_val_val eptr)). {
+    simpl. auto.
+  } rewrite <- memory_block_data_at_; auto.
+} rewrite H1. clear H1.
+assert (data_at_ sh (tarray t_struct_edge MAX_EDGES) (pointer_val_val eptr) = data_at sh (tarray t_struct_edge MAX_EDGES) (list_repeat (Z.to_nat MAX_EDGES) (Vundef, (Vundef, Vundef))) (pointer_val_val eptr)). {
+  unfold data_at_, field_at_, data_at. assert (default_val (nested_field_type (tarray t_struct_edge MAX_EDGES) []) = list_repeat (Z.to_nat MAX_EDGES) (Vundef, (Vundef, Vundef))) by reflexivity.
+  rewrite H1. auto.
+} rewrite H1. clear H1.
+forward.
+forward.
+forward.
+forward.
+forward.
+Exists empty_WEdgeListGraph_finite gptr eptr.
+unfold wedgearray_graph_rep.
+rewrite empty_WEdgeListGraph_numV. rewrite empty_WEdgeListGraph_numE.
+simpl. rewrite data_at_zero_array_eq. entailer!.
+reflexivity. apply H4. rewrite empty_WEdgeListGraph_graph_to_wedgelist. simpl. reflexivity.
+Qed.
 
 Definition kruskal_spec :=
   DECLARE _kruskal
-  WITH sh: wshare, g: WeightedEdgeListGraph.LGraph, pointer_g : pointer_val
+  WITH gv: globals, sh: wshare, g: WEdgeListGraph, gptr : pointer_val, eptr : pointer_val
   PRE [tptr t_wedgearray_graph]
-   PROP (sound_weighted_edge_graph g;
-         (numE g) <= SIZE
+   PROP (sound_weighted_edge_graph g; numE g <= MAX_EDGES
         )
-   PARAMS ((pointer_val_val pointer_g))
-   GLOBALS ()
-   SEP (graph_rep sh g (pointer_val_val pointer_g))
+   PARAMS ((pointer_val_val gptr))
+   GLOBALS (gv)
+   SEP (data_at sh tint (Vint (Int.repr MAX_EDGES)) (gv _MAX_EDGES);
+        wedgearray_graph_rep sh g gptr eptr)
   POST [tptr t_wedgearray_graph]
    EX pointer_msf: pointer_val,
-   EX (msf: WeightedEdgeListGraph.LGraph) {f_msf: FiniteGraph msf},
-   PROP (sound_weighted_edge_graph msf;
+   EX (msf: WEdgeListGraph) {f_msf: FiniteGraph msf},
+   PROP (sound_weighted_edge_graph msf; (numE msf) <= MAX_EDGES;
          minimum_spanning_forest g msf)
    LOCAL (temp ret_temp pointer_msf)
-   SEP (graph_rep sh g (pointer_val_val pointer_g);
-        graph_rep sh msf pointer_msf).
+   SEP (data_at sh tint (Vint (Int.repr MAX_EDGES)) (gv _MAX_EDGES);
+        wedgearray_graph_rep sh g (pointer_val_val gptr);
+        wedgearray_graph_rep sh msf pointer_msf).
+
+(*
+Idea of proof:
+int graph_V = graph->V;
+int graph_E = graph->E;
+struct subset *subsets = makeSet(graph_V); (*ufgraph with V vertices all distinct*)
+struct graph *mst = init_empty_graph();
+
+mst->V = graph_V; <-- mst is now a graph with V vertices and 0 edges
+
+sort_edges(graph->edge_list,0,graph_E-1);
+
+    //invariant: is_partial_graph mst orig_graph /\ uforest mst
+    //   connected ufgraph u v <-> connected in mst (also connected ufgraph u v -> connected graph u v)
+    // showing forest is a problem... need an easy-to-work-with definition
+    // and something about minimum weight...
+    //precon: mst has no edges, is a trivial subset, trivial forest. subsets are all disjoint
+    for (int i = 0; i < graph_E; ++i) {
+
+        int u = graph->edge_list[i].u;
+        int v = graph->edge_list[i].v;
+
+        int ufind = find(subsets, u);		//returned g' is: uf_root g' i rt
+        int vfind = find(subsets, v);
+
+        //need a join postcon?
+        //ufind != vfind <-> not connected in mst
+        //not_connected -> add edge -> no cycle <-- Need a lemma in undirected_graph.v
+        //also show that edge here: minimum of all (u,v) edges
+        if (ufind != vfind) {
+            mst->edge_list[mst->E].u = u;
+            mst->edge_list[mst->E].v = v;
+            mst->edge_list[mst->E].weight = graph->edge_list[i].weight;
+            mst->E += 1;
+            Union(subsets, u, v);
+
+            //mst = mst + (u,v), thus u,v are connected
+            //ifcon (loopcon): is_partial_graph (mst + (u,v)) orig
+            //mst is still uforest (using the needed lemma above)
+            //same_subset(u,v) /\ u,v connected (*trivially <->*)
+        }
+        //need an elsecon?
+        //uf_root p u -> reachable g u p -> connected p u (reachable_implies_connected)
+        //connected p u -> connected p v -> connected u v (connected_trans)
+    }
+    //postcon
+
+    //before free, need to prove that same_subset(u,v) <-> connected orig u v
+    //from invariant, same_subset(u,v) <-> connected in mst
+    //thus, connected in mst <-> connected in orig: spanning definition
+
+    free(subsets);
+
+    //worried about proving minimum
+    return mst;
 
 *)
